BSM to MM done

theories/MinskyMachines/Reductions/BSM_computable_to_MM_computable.v
@@ -34,6 +34,12 @@ Proof.
   destruct E. cbn. now rewrite !cast_eq_refl.
 Qed.
 
+Lemma MM_cast_terminates {n m} i (P : list (mm_instr (pos n))) (E : n = m) j v :
+   sss.sss_terminates (@mm_sss _) (i, P) (j, v) <-> sss.sss_terminates (@mm_sss _) (i, MM_cast P E) (j, Vector.cast v E).
+Proof.
+  destruct E. cbn. now rewrite !cast_eq_refl.
+Qed.
+
 Local Notation "P '/MM/' s '~~>' t" := (sss.sss_output (@mm_sss _) P s t) (at level 70, no associativity).
 Local Notation "P '/MM/' s '~~>' t" := (sss.sss_output (@mm_sss _) P s t) (at level 70, no associativity).
 
@@ -49,6 +55,11 @@ Proof.
   - rewrite vec_app_cons. cbn. congruence.
 Qed.
 
+Lemma vec_map_spec {X Y n} (v : Vector.t X n) (f : X -> Y) :
+  vec_map f v = Vector.map f v.
+Proof.
+  induction v; cbn; congruence.
+Qed.
 
 Lemma vec_change_swap [X] [n] (v : vec X n) (p : pos n) (q : pos n) x y :
 p <> q ->
@@ -162,7 +173,13 @@ Qed.
 Lemma vector_inv_back {X n} (v : Vector.t X (S n)) E :
   { '(x, v') : X * Vector.t X n | v = Vector.cast (append v' (x ## vec_nil)) E }.
 Proof.
-Admitted.
+  destruct E. 
+  destruct (splitat n v) eqn:E.
+  eexists (vec_head t0, t).
+  erewrite <- append_splitat. now rewrite cast_eq_refl.
+  rewrite E. f_equal. eapply (Vector.caseS' t0). cbn.
+  intros h. eapply Vector.case0. reflexivity.
+Qed.
 
 Lemma pos_left_spec {m n} p :
   @pos_left m n p = Fin.L n p.
@@ -197,14 +214,20 @@ Proof.
     + rewrite IHl1. reflexivity. lia.
 Qed.
 
+Lemma vec_list_const {X x n} : vec_list (@const X x n) = List.repeat x n.
+Proof. induction n; cbn; congruence. Qed.
+
 Section preprocess.
 
   Variables k n : nat.
 
-  Notation reg p := (@pos_left (1 + k + n) 2 (pos_left n (pos_right 1 p))).
-  Notation tmp p := (@pos_right (1 + k + n) 2 p).
+  Notation reg p := (@pos_left (1 + k + n) 3 (pos_left n (pos_right 1 p))).
+  Notation tmp p := (@pos_right (1 + k + n) 3 p).
 
   Lemma tmp0_tmp1 : tmp pos0 <> tmp pos1. Proof. intros H % pos_right_inj. congruence. Qed.
+  Lemma tmp0_tmp2 : tmp pos0 <> tmp pos2. Proof. intros H % pos_right_inj. congruence. Qed.
+  Lemma tmp2_tmp0 : tmp pos2 <> tmp pos0. Proof. intros H % pos_right_inj. congruence. Qed.
+  Lemma tmp1_tmp2 : tmp pos1 <> tmp pos2. Proof. intros H % pos_right_inj % pos_nxt_inj. congruence.  Qed.
 
   Lemma tmp_tgt p : tmp p <> pos0. Proof. cbn. congruence. Qed.
 
@@ -214,13 +237,13 @@ Section preprocess.
 
   Lemma reg_inj p q : reg p = reg q -> p = q. Proof. cbn. now intros ? % pos_nxt_inj % pos_left_inj % pos_left_inj. Qed.
 
-  Hint Resolve tmp0_tmp1 tmp_tgt tmp_reg tgt_reg reg_inj : core.
+  Hint Resolve tmp0_tmp1 tmp0_tmp1 tmp2_tmp0 tmp1_tmp2 tmp_tgt tmp_reg tgt_reg reg_inj : core.
 
   Section prep.
 
   Import ListNotations.
 
-  Definition prep (p : pos k) (i : nat) : list (mm_instr (pos (1 + k + n + 2))) := 
+  Definition prep (p : pos k) (i : nat) : list (mm_instr (pos (1 + k + n + 3))) := 
   (* i: *)    mm_transfert (reg p) pos0 (tmp pos0) i ++
   (* i+3: *) [INC (reg p)] ++
   (* i+4: *) [DEC Fin.F1 (14 + i)] ++ 
@@ -243,7 +266,7 @@ Section preprocess.
     eapply sss_compute_trans.
     { eapply subcode_sss_compute with (P := (i,mm_transfert (reg p) (pos0) (pos_right (1 + k + n) Fin.F1) i)). auto.
       eapply sss_progress_compute. eapply mm_transfert_progress; auto. }
-    mm sss INC with (pos_left 2 (pos_left n (pos_right 1 p))). replace (3 + i) with (i + 3) by lia. auto.
+    mm sss INC with (pos_left 3 (pos_left n (pos_right 1 p))). replace (3 + i) with (i + 3) by lia. auto.
     rew vec. replace (1 + (3 + i)) with (4 + i) by lia.
     rewrite vec_change_swap.
     rewrite vec_change_idem. 
@@ -267,7 +290,7 @@ Section preprocess.
         mm sss stop. }
       rew vec.
       eapply sss_compute_trans.
-      { eapply subcode_sss_compute with (P := (5 + i, mm_push_One (pos_left 2 (pos_left n (pos_right 1 p))) (pos_right (1 + k + n) pos0) (pos_right (1 + k + n) pos1) (5+i))).
+      { eapply subcode_sss_compute with (P := (5 + i, mm_push_One (pos_left 3 (pos_left n (pos_right 1 p))) (pos_right (1 + k + n) pos0) (pos_right (1 + k + n) pos1) (5+i))).
         1: replace (5 + i) with (i + 5) at 1 by lia; auto.
         eapply sss_progress_compute. eapply mm_push_One_progress; rew vec.
         - rewrite vec_change_neq; eauto.
@@ -281,7 +304,7 @@ Section preprocess.
       lia. assumption.
   Qed.
 
-  Fixpoint PREP' (k' : nat) (H : k' <= k) (i : nat) : list (mm_instr (pos (1 + k + n + 2))).
+  Fixpoint PREP' (k' : nat) (H : k' <= k) (i : nat) : list (mm_instr (pos (1 + k + n + 3))).
   Proof.
     destruct k'.
     - exact List.nil.
@@ -297,7 +320,7 @@ Section preprocess.
     - autorewrite with list. rewrite IHk'. cbn. lia.
   Qed.
 
-  Definition PREP (i : nat) : list (mm_instr (pos (1 + k + n + 2))). refine (@PREP' k _ i). abstract lia. Defined.
+  Definition PREP (i : nat) : list (mm_instr (pos (1 + k + n + 3))). refine (@PREP' k _ i). abstract lia. Defined.
 
   Lemma PREP_length i : length (PREP i) = k * 14. Proof. eapply PREP'_length. Qed.
   Hint Resolve PREP_length : core.    
@@ -307,8 +330,8 @@ Section preprocess.
     v = (Vector.cast (Vector.append v1 v2) E) ->
     x = 0 ->
     forall H,
-    (i, PREP' k'' H i) /MM/ (i, Vector.append (Vector.append (x ## v) w) (0 ## 0 ## vec_nil)) ~~>
-    (i + (k'' * 14), Vector.append (Vector.append (x ## (Vector.cast (Vector.append (Vector.map (fun n => stack_enc (List.repeat true n)) v1) v2) E)) w) (0 ## 0 ## vec_nil)).
+    (i, PREP' k'' H i) /MM/ (i, Vector.append (Vector.append (x ## v) w) (0 ## 0 ## 0 ## vec_nil)) ~~>
+    (i + (k'' * 14), Vector.append (Vector.append (x ## (Vector.cast (Vector.append (Vector.map (fun n => stack_enc (List.repeat true n)) v1) v2) E)) w) (0 ## 0 ## 0 ## vec_nil)).
   Proof. 
     intros E -> -> Hle. 
     split. 2:{ cbn. rewrite PREP'_length. right. lia. }
@@ -321,7 +344,7 @@ Section preprocess.
       assert (H2 : k'' + S k' = k) by lia.
       specialize (IHk'' i v1l (S k') (PREP'_subproof k'' Hle) H2 (x ## v2)).
       eapply subcode_sss_compute_trans with (P := (i, PREP' k'' (PREP'_subproof k'' Hle) i)). auto.
-      match type of IHk'' with sss_compute _ _ (_, ?st) _ => evar (Vector.t nat (1 + k + n + 2)); enough (Eq : st = t) end; subst t.
+      match type of IHk'' with sss_compute _ _ (_, ?st) _ => evar (Vector.t nat (1 + k + n + 3)); enough (Eq : st = t) end; subst t.
       rewrite Eq in IHk''. eapply IHk''.
       { rewrite Hv1. repeat f_equal.
         eapply vec_list_inj. rewrite !vec_list_cast, <- !vec_app_spec, !vec_list_vec_app.
@@ -340,7 +363,7 @@ Section preprocess.
         eapply vec_list_inj.
         
         rewrite vec_list_vec_change.
-        rewrite !(@vec_list_vec_app nat (1 + k + n) 2).
+        rewrite !(@vec_list_vec_app nat (1 + k + n) 3).
         rewrite !vec_list_vec_app. cbn [vec_list].
         rewrite !vec_list_cast.
         rewrite !vec_list_vec_app. cbn [vec_list].
@@ -348,7 +371,7 @@ Section preprocess.
         rewrite <- !vec_app_spec.
         rewrite !vec_list_vec_app. cbn [vec_list].
         clear. fold plus.
-        rewrite pos_left_spec. pose proof (@Fin.L_sanity (S (k + n)) 2). cbn in H. rewrite H. clear H.
+        rewrite pos_left_spec. pose proof (@Fin.L_sanity (S (k + n)) 3). cbn in H. rewrite H. clear H.
         rewrite pos_left_spec. pose proof (@Fin.L_sanity (S (k)) n). cbn in H. rewrite H. clear H.
         rewrite pos_right_spec. pose proof (@Fin.R_sanity k 1 ). cbn [plus] in H. rewrite H. clear H.
         rewrite Fin.to_nat_of_nat. cbn [proj1_sig update app]. f_equal.
@@ -361,7 +384,7 @@ Section preprocess.
         f_equal. f_equal.
         rewrite <- !app_assoc. f_equal.
         cbn [app]. f_equal. f_equal. f_equal.
-        rewrite (@vec_pos_app_left nat (add (S k) n) 2).
+        rewrite (@vec_pos_app_left nat (add (S k) n) 3).
         rewrite <- pos_left_spec.
         rewrite (@vec_pos_app_left nat (S k) n).
         rewrite <- pos_right_spec.
@@ -381,12 +404,12 @@ Section preprocess.
   Defined.
 
   Lemma PREP_spec i v w :
-      (i, PREP i) /MM/ (i, Vector.append (Vector.append (0 ## v) w) (0 ## 0 ## vec_nil)) ~~> (i + (k * 14), Vector.append (Vector.append (0 ## Vector.map (fun n => stack_enc (List.repeat true n)) v) w) (0 ## 0 ## vec_nil)).
+      (i, PREP i) /MM/ (i, Vector.append (Vector.append (0 ## v) w) (0 ## 0 ## 0 ## vec_nil)) ~~> (i + (k * 14), Vector.append (Vector.append (0 ## Vector.map (fun n => stack_enc (List.repeat true n)) v) w) (0 ## 0 ## 0 ## vec_nil)).
   Proof.
     unfold PREP.
     pose proof (@PREP_spec_strong i 0 w k 0 v vec_nil v (myeq k)).
-    match goal with [ |- sss_output _ _ (_, ?st) _ ] => evar (Vector.t nat (1 + k + n + 2)); enough (st = t) as ->; subst t end.
-    match goal with [ |- sss_output _ _ _ (_, ?st) ] => evar (Vector.t nat (1 + k + n + 2)); enough (st = t) as ->; subst t end.
+    match goal with [ |- sss_output _ _ (_, ?st) _ ] => evar (Vector.t nat (1 + k + n + 3)); enough (st = t) as ->; subst t end.
+    match goal with [ |- sss_output _ _ _ (_, ?st) ] => evar (Vector.t nat (1 + k + n + 3)); enough (st = t) as ->; subst t end.
     eapply H; try reflexivity. 3: reflexivity.
     2:{ repeat f_equal. clear. induction k; cbn. 
         - rewrite cast_eq_refl.
@@ -400,13 +423,169 @@ Section preprocess.
     - cbn. f_equal. eapply IHv.
   Qed.
 
-  Definition POSTP (i : nat) : list (mm_instr (pos (1 + k + n + 2))) := @List.nil _.
+  Fixpoint PREPMORE' (n' : nat) (H : n' <= n) : list (mm_instr (pos (1 + k + n + 3))).
+  Proof.
+    destruct n'.
+    - exact List.nil.
+    - refine (List.app (PREPMORE' n' _) _). abstract lia.
+      assert (Hn : n' < n) by abstract lia.
+      refine (INC (pos_left 3 (pos_right (1 + k) (Fin.of_nat_lt Hn))) :: List.nil).
+  Defined. 
+
+  Lemma PREPMORE'_length (n' : nat) (H : n' <= n) : length (PREPMORE' n' H) = n'.
+  Proof.
+    induction n' in H |- *; cbn.
+    - reflexivity.
+    - simpl_list. rewrite IHn'. cbn. lia.
+  Qed.
+
+  Definition PREPMORE : list (mm_instr (pos (1 + k + n + 3))). refine (@PREPMORE' n _). abstract lia. Defined.
+
+  Lemma PREPMORE'_spec i x (w : Vector.t nat k) n'' n' :
+    forall E : n'' + n' = n,
+    forall H,
+    (i, PREPMORE' n'' H) /MM/ (i, Vector.append (Vector.append (x ## w) (Vector.const 0 n)) (0 ## 0 ## 0 ## vec_nil)) ~~> 
+    (i + n'', Vector.append (Vector.append (x ## w) (Vector.cast (Vector.append (Vector.const 1 n'') (Vector.const 0 n')) E)) (0 ## 0 ## 0 ## vec_nil)).
+  Proof.
+    intros E Hle.
+    split. 2:{ cbn. rewrite PREPMORE'_length. lia. }
+    revert n' E Hle.
+    induction n''; intros n' E Hle.
+    - cbn [PREPMORE']. mm sss stop. f_equal. lia. repeat f_equal. cbn. destruct E. now rewrite cast_eq_refl.
+    - cbn [PREPMORE'].
+      eapply subcode_sss_compute_trans with (P := (i, PREPMORE' n'' (PREPMORE'_subproof n'' Hle))). auto.
+      { eapply IHn''. }
+      mm sss INC with (pos_left 3 (pos_right (1 + k) (Fin.of_nat_lt (PREPMORE'_subproof0 n'' Hle)))).
+      { eexists. eexists. split. reflexivity. now rewrite PREPMORE'_length. }
+      mm sss stop. f_equal. 1: lia.
+      rewrite <- !vec_app_spec.
+      rewrite !vec_pos_app_left.
+      rewrite !vec_pos_app_right.
+      eapply vec_list_inj. 
+      rewrite vec_list_vec_change.
+      rewrite !vec_list_vec_app.
+      rewrite pos_left_spec.
+      rewrite Fin.L_sanity.
+      rewrite pos_right_spec.
+      rewrite Fin.R_sanity.
+      rewrite Fin.to_nat_of_nat. cbn [proj1_sig plus].
+      rewrite update_app_left. 2:{ rewrite !app_length, !vec_list_length. lia. }
+      f_equal.
+      rewrite update_app_right. 2:{ cbn. rewrite !vec_list_length. lia. }
+      f_equal. rewrite vec_list_length. replace (S (k + n'') - S k) with n'' by lia.
+      rewrite !vec_list_cast.
+      rewrite !vec_list_vec_app.
+      rewrite update_app_right. 2:{ cbn. rewrite !vec_list_length. lia. }
+      rewrite (@vec_list_vec_app nat (S n'') n').
+      replace (S n'') with (n'' + 1) by lia.
+      rewrite vec_list_length. rewrite minus_diag. instantiate (2 := 1 + n'). cbn.
+      rewrite !vec_list_const. rewrite repeat_app. cbn. rewrite <- !app_assoc.
+      f_equal. cbn. f_equal.
+      f_equal.
+      eapply nth_error_vec_list.
+      rewrite vec_list_cast, !vec_list_vec_app; cbn. 
+      rewrite nth_error_app2. 2: rewrite vec_list_length; lia.
+      now rewrite vec_list_length, minus_diag.
+      Unshelve. lia.
+  Qed.
+
+  Lemma PREPMORE_spec i x (w : Vector.t nat k) :
+    (i, PREPMORE) /MM/ (i, Vector.append (Vector.append (x ## w) (Vector.const 0 n)) (0 ## 0 ## 0 ## vec_nil)) ~~> 
+    (i + n, Vector.append (Vector.append (x ## w) (Vector.const 1 n)) (0 ## 0 ## 0 ## vec_nil)).
+  Proof.
+    pose proof (PREPMORE'_spec i x w n 0). cbn in H. cbn.
+    match goal with [ |- sss_output _ _ _ (_, ?st) ] => evar (Vector.t nat (1 + k + n + 3)); enough (st = t) as ->; subst t end.
+    eapply H. repeat f_equal.
+    eapply vec_list_inj. rewrite vec_list_cast, vec_list_const, <- vec_app_spec, vec_list_vec_app, vec_list_const.
+    now simpl_list.
+    Unshelve. lia.
+  Qed.
+
+  Section POSTP.
+  Import ListNotations.
+
+  Definition POSTP (i : nat) : list (mm_instr (pos (1 + k + n + 3))) := 
+(*     (*    i *) mm_transfert pos0 (tmp pos2) (tmp pos0) i ++
+ *) (*    i *) mm_pop (tmp pos2) (tmp pos0) (tmp pos1) (i) (i+16) (i+16) (i+18) ++
+    (* 16+i *)[INC pos0] ++
+    (* 17+i *)[DEC (tmp pos0) (i)].
+    
+  End POSTP.
+
+  Lemma POSTP_length i : length (POSTP i) = 18. Proof. reflexivity. Qed.
+  Hint Resolve POSTP_length : core.
+  Hint Rewrite POSTP_length : list.
+
+  Lemma POSTP_spec_strong i v out out' :
+     v #> pos0 = out' ->
+     v #> tmp pos0 = 0 ->
+     v #> tmp pos1 = 0 ->
+     v #> tmp pos2 = stack_enc (List.repeat true out) ->
+     (i, POSTP i) /MM/ (i, v) ~~> (i + 18, v [ (out + out') / Fin.F1 ] [ (stack_enc nil) / tmp pos2] ).
+  Proof.
+    intros Htgt Htmp0 Htmp1 Htmp2.
+    split. 2:{ cbn. lia. }
+    induction out in v, Htgt, Htmp0, Htmp1, Htmp2, out', Htgt, Htmp2 |- *.
+    - cbn [repeat] in Htmp2. 
+      eapply subcode_sss_compute_trans with (P := (i,mm_pop (tmp pos2) (tmp pos0) (tmp pos1) (i) (i+16) (i+16) (i+18))). 1: unfold POSTP; auto.
+      { eapply sss_progress_compute. eapply mm_pop_void_progress; eauto. }
+      mm sss stop. f_equal. eapply vec_pos_ext. fold plus. intros p.
+      eapply (Fin.caseS' p).
+      + rewrite vec_change_neq; eauto. rewrite vec_change_eq; eauto.
+      + clear p. apply pos_left_right_rect.
+        * intros p. rewrite !vec_change_neq; try congruence. intros ? % pos_nxt_inj. fold pos_right in H0. eapply pos_right_left. now rewrite H0. 
+        * intros p. eapply (Fin.caseS' p); clear p.
+          -- rewrite !vec_change_neq; try congruence. eapply tmp2_tmp0.
+          -- intros p. eapply (Fin.caseS' p); clear p.
+             ++ rewrite !vec_change_neq; try congruence. intros H. eapply tmp1_tmp2. cbn. rewrite <- H. reflexivity.
+             ++ intros p. eapply (Fin.caseS' p); clear p.
+               ** rewrite vec_change_eq. 2: reflexivity. eauto.
+               ** eapply Fin.case0.
+    - cbn [repeat] in Htmp2. 
+      eapply subcode_sss_compute_trans with (P := (i,mm_pop (tmp pos2) (tmp pos0) (tmp pos1) (i) (i+16) (i+16) (i+18))). 1: unfold POSTP; auto.
+      { eapply sss_progress_compute. eapply mm_pop_One_progress; eauto. }
+      mm sss INC with pos0. unfold POSTP. auto. fold plus in *.
+      mm sss DEC 0 with (tmp pos0) i. unfold POSTP. auto. 
+      {rew vec. rewrite vec_change_neq; eauto. }
+      rew vec. specialize IHout with (out' := S out'). 
+      replace (out + S out') with (S (out + out')) in IHout by lia.
+      match goal with [ |- sss_compute _ _ _ (_, ?st) ] => evar (Vector.t nat (1 + k + n + 3)); enough (st = t) as ->; subst t end.
+      eapply IHout; rew vec.
+      + rewrite vec_change_neq; eauto.
+      + rewrite vec_change_neq; eauto.
+      + rew vec. symmetry. rewrite vec_change_swap. 2: eauto. rewrite vec_change_idem, vec_change_swap; eauto.
+  Qed.
 
   Lemma POSTP_spec i v out :
-     v #> pos_right (1 + k + n) Fin.F1 = 0 ->
-     v #> Fin.F1 = stack_enc (List.repeat true out) ->
-     (i, POSTP i) /MM/ (i, v) ~~> (i + 3, v [ out / Fin.F1 ]).
-  Admitted.
+     v #> pos0 = 0 ->
+     v #> tmp pos0 = 0 ->
+     v #> tmp pos1 = 0 ->
+     v #> tmp pos2 = stack_enc (List.repeat true out) ->
+     (i, POSTP i) /MM/ (i, v) ~~> (i + 18, v [ out / pos0] [ (stack_enc nil) / tmp pos2 ]).
+  Proof.
+    intros Htgt Htmp0 Htmp1 Htmp2.
+    pose proof (POSTP_spec_strong i v out 0 Htgt Htmp0 Htmp1 Htmp2). rewrite NPeano.Nat.add_0_r in H.
+    eapply H.
+  Qed.
+
+  Definition PREPALL i := PREP i ++ PREPMORE ++ INC pos0 :: List.nil.
+
+  Lemma PREPALL_length i : length (PREPALL i) = k * 14 + n + 1.
+  Proof. unfold PREPALL, PREPMORE; rewrite !app_length, PREP_length, PREPMORE'_length; cbn; lia. Qed.
+
+  Lemma PREPALL_spec i v : 
+    (i, PREPALL i) /MM/ (i, Vector.append (Vector.append (0 ## v) (Vector.const 0 n)) (0 ## 0 ## 0 ## vec_nil)) ~~>
+          (i + k * 14 + n + 1, Vector.append (Vector.append (stack_enc nil ## Vector.map (fun n => stack_enc (List.repeat true n)) v) (Vector.const (stack_enc nil) n)) (0 ## 0 ## 0 ## vec_nil)).
+  Proof.
+    split. 2: cbn; rewrite PREPALL_length; lia.
+    eapply subcode_sss_compute_trans. 2: eapply PREP_spec. 1: unfold PREPALL; auto.
+    eapply subcode_sss_compute_trans. 2: eapply PREPMORE_spec. 1: unfold PREPALL; auto.
+    mm sss INC with pos0.
+    { unfold PREPALL. eexists. eexists nil. cbn. split. now rewrite app_assoc.
+      rewrite app_length, PREP_length; unfold PREPMORE; rewrite PREPMORE'_length. lia. }
+    fold plus. mm sss stop.
+    f_equal. lia.
+  Qed.
 
 End preprocess.
 
@@ -416,49 +595,57 @@ Proof.
   destruct E. now rewrite !cast_eq_refl.
 Qed.
 
-Definition cases {k i} : (forall p : pos (1 + k + i + 2),
-{p = pos_right (1 + k + i) pos0} + {p = pos_right (1 + k + i) pos1} +
-{q : pos (1 + k + i) | p = pos_left 2 q}).
+Definition cases {k i} : (forall p : pos (1 + k + i + 3),
+{p = pos_right (1 + k + i) pos0} + {p = pos_right (1 + k + i) pos1} + {p = pos_right (1 + k + i) pos2} +
+{q : pos (1 + k + i) | p = pos_left 3 q}).
 Proof.
   apply pos_left_right_rect; [ eauto | ].
   intros p. eapply (Fin.caseS' p); [ eauto | ].
   intros p'. eapply (Fin.caseS' p'); [ eauto | ].
+  intros p''. eapply (Fin.caseS' p''); [ eauto | ].
   eapply Fin.case0.
 Defined.
 
-Lemma MM_computable_to_BSM_computable {k} (R : Vector.t nat k -> nat -> Prop) :
+Lemma vec_pos_const {k} {X x} (p : pos k) : @const X x k #> p = x.
+Proof.
+  induction p; cbn; eauto.
+Qed.
+
+Lemma BSM_computable_to_MM_computable {k} (R : Vector.t nat k -> nat -> Prop) :
   BSM_computable R -> MM_computable R.
 Proof.
-  intros (i & n & P & HP). red.
-  unshelve epose proof (@bsm_mm_compiler_strong (1 + k + i) n P (pos_right _ Fin.F1) (pos_right _ (Fin.FS Fin.F1)) (pos_left _) (1 + length (PREP k i 1)) _ _ _ _ ) as [Q HQ]. 
+  intros (i & n & P & HP1 & HP2) % BSM_computable_iff. eapply MM_computable_iff.
+  unshelve epose proof (@bsm_mm_compiler_strong (1 + k + i) n P (pos_right _ Fin.F1) (pos_right _ (Fin.FS Fin.F1)) (pos_right _ (pos2)) (pos_left _) (1 + length (PREPALL k i 1)) _ _ _ _ ) as [Q HQ].
   - eapply tmp0_tmp1.
   - intros p. intros H. eapply  pos_right_left. now rewrite H.
   - intros.  intros H. eapply  pos_right_left. now rewrite H.
   - now intros ? ? ? % pos_left_inj.
   - exact cases.
-  - exists (i + 2). assert (E : 1 + k + i + 2 = (1 + k) + (i + 2)) by lia.
-    pose (q' := (List.app (List.app (PREP k i 1) Q) (POSTP k i 20))).
-    exists (MM_cast q' E). fold plus.
-    intros v m. etransitivity. 
-    { split. intros ? % HP. exact H0. eapply HP. }
-    assert (Eq1 : cast (append (append (0 ## v) (const 0 i)) (const 0 2)) E = append (0 ## v) (const 0 (i + 2))).
-    { clear. cbn.
-      f_equal. match goal with [ |- context [@f_equal ?A ?B ?f ?x ?y ?e]] => generalize (@f_equal A B f x y e) end. clear.
-      induction v; cbn; intros E.
-      - induction i in E |- *; cbn.
-        + reflexivity.
-        + now rewrite IHi.
-      - f_equal. now rewrite IHv.
-    }
-    setoid_rewrite eval_iff. split.
-    + intros (c & v' & H % BSM_sss.eval_iff). fold plus in *.
+  - intros ? % pos_right_inj; congruence.
+  - intros ? % pos_right_inj % pos_nxt_inj. congruence.
+  - intros p. intros H. eapply  pos_right_left. now rewrite H.
+  - exists (i + 3).   assert (E : 1 + k + i + 3 = (1 + k) + (i + 3)) by lia.
+    pose (q' := PREPALL k i 1 ++ Q ++ mm_transfert pos0 (pos_right (1 + k + i) pos2) (pos_right (1 + k + i) pos0) (1 + length (PREPALL k i 1) + length Q) ++ POSTP k i (4 + length (PREPALL k i 1) + length Q)).
+    assert (Eq1 : forall v, cast (append (append (0 ## v) (const 0 i)) (const 0 3)) E = append (0 ## v) (const 0 (i + 3))).
+      { intros v. clear. cbn.
+        f_equal. match goal with [ |- context [@f_equal ?A ?B ?f ?x ?y ?e]] => generalize (@f_equal A B f x y e) end. clear.
+        induction v; cbn; intros E.
+        - induction i in E |- *; cbn.
+          + reflexivity.
+          + now rewrite IHi.
+        - f_equal. now rewrite IHv.
+      }
+    exists (MM_cast q' E). fold plus. split.
+    + intros v m. intros ? % HP1.
+      setoid_rewrite eval_iff.
+      destruct H0 as (c & v' & H % BSM_sss.eval_iff). fold plus in *.
       eapply HQ in H. 
       eexists. eexists ?[v']. rewrite <- Eq1.
-      unshelve eassert (Eq2 : forall v' : Vector.t nat (k + (i + 2)), m ## v' = cast (m ## _) E).
+      unshelve eassert (Eq2 : forall v' : Vector.t nat (k + (i + 3)), m ## v' = cast (m ## _) E).
       { fold plus. refine (Vector.cast v' _). abstract lia. }
       { clear. intros v. cbn. f_equal.
         match goal with [ |- context [@f_equal ?A ?B ?f ?x ?y ?e]] => generalize (@f_equal A B f x y e) end. fold plus.
-        intros E2. generalize (MM_computable_to_BSM_computable_subproof k i E).
+        intros E2. generalize (BSM_computable_to_MM_computable_subproof k i E).
         clear. intros E1. cbn in *. revert v E1 E2. generalize (k + i + 2).  generalize (k + (i + 2)). clear. intros.
         destruct E1. now rewrite !cast_eq_refl.
       }
@@ -466,29 +653,115 @@ Proof.
       instantiate (v' := (cast _ _)).
       rewrite <- @MM_cast_spec. subst q'.
       split. 
-      1: { eapply subcode_sss_compute_trans. 2: eapply PREP_spec. 1: auto.
-      match goal with [H : sss_output _  _ ?st1 _ |- sss_compute _ _ ?st2 _ ] => assert (st1 = st2) by admit end.
+      1: { eapply subcode_sss_compute_trans. 2: eapply PREPALL_spec. 1: auto.
+      match goal with [H : sss_output _  _ ?st1 _ |- sss_compute _ _ ?st2 _ ] => enough (st1 = st2) end.
       rewrite H0 in H.
       eapply subcode_sss_compute_trans. 2: eapply H. auto.
-      unfold vec_enc. unfold vec_set_pos. cbn [plus].
-      destruct cases as [ [ | ] | [q Hq]]. 
-      1:{ cbn in *. congruence.  }
-      1:{ cbn in *; congruence. }
-      revert Hq. eapply (Fin.caseS' q).
-      2:{ cbn. congruence. }
-      intros _. clear q.
-      eapply subcode_sss_compute_trans. 2: eapply POSTP_spec. admit.
-      { cbn. rewrite vec_pos_set. destruct cases as [ [ | ] | [q Hq]]. 
-      1:{ cbn in *. congruence.  }
-      1:{ cbn in *; congruence. }
-      revert Hq. eapply (Fin.caseS' q).
-      2:{ cbn. intros ? ? % pos_nxt_inj. exfalso. eapply pos_right_left. now rewrite H1. }
-      clear H. cbn. congruence.
+      2:{ f_equal. rewrite PREPALL_length. lia. clear.
+          eapply vec_pos_ext. intros p.
+          unfold vec_enc. rewrite vec_pos_set. destruct (cases p) as [ [[-> | ->] | ->] | [q ->]].
+          - cbn. rewrite <- !vec_app_spec. now rewrite vec_pos_app_right.
+          - cbn. rewrite <- !vec_app_spec. now rewrite vec_pos_app_right.
+          - cbn. rewrite <- !vec_app_spec. now rewrite vec_pos_app_right.
+          - rewrite <- !vec_app_spec. rewrite vec_pos_app_left.
+            revert q. eapply pos_left_right_rect.
+            + intros p. rewrite !vec_pos_app_left.
+              rewrite <- !vec_map_spec. eapply (Fin.caseS' p).
+              * cbn. reflexivity.
+              * cbn. intros. rewrite !vec_pos_map. reflexivity.
+            + intros p. rewrite !vec_pos_app_right.
+              now rewrite !vec_pos_const.
       }
-      { cbn. reflexivity. }
+      eapply subcode_sss_compute_trans with (P := (1 + length (PREPALL k i 1) + length Q, mm_transfert pos0 (pos_right (1 + k + i) pos2) (pos_right (1 + k + i) pos0) (1 + length (PREPALL k i 1) + length Q))).
+      { eexists (PREPALL k i 1 ++ Q). eexists (POSTP _ _ _). split. now rewrite <- app_assoc. rewrite !app_length, PREPALL_length. lia. }
+      eapply sss_progress_compute. eapply mm_transfert_progress.
+      1-5: clear.
+      { cbn. congruence. }
+      { cbn. congruence. } 
+      { cbn. intros ? % pos_nxt_inj % pos_right_inj. congruence. }
+      { unfold vec_enc. rewrite vec_pos_set.
+        destruct cases as [ [ [| ] | ] | [q Hq]]; rew vec.
+        exfalso. eapply pos_right_left. now rewrite Hq. }
+      { unfold vec_enc. rewrite vec_pos_set. 
+        destruct cases as [ [ [| ] | ] | [q Hq]]; rew vec.
+        exfalso. eapply pos_right_left. now rewrite Hq. }
+      { reflexivity. }
+      eapply subcode_sss_compute_trans with (P := (4 + length (PREPALL k i 1) + length Q, POSTP k i (4 + length (PREPALL k i 1) + length Q))).
+      { eexists _. eexists List.nil. split. rewrite app_nil_r. now rewrite !app_assoc. rewrite !app_length, PREPALL_length. cbn. lia. }
+      eapply POSTP_spec.
+      { unfold vec_enc. rewrite vec_pos_set. destruct cases as [ [ | ] | [q Hq]]; rew vec. }
+      { unfold vec_enc. rewrite !vec_pos_set.
+        destruct cases as [ [ [| ] | ] | [q Hq]]; rew vec.
+        all: try now (cbn in e; congruence).
+        revert Hq. eapply (Fin.caseS' q).
+        all: try now (cbn; congruence).
+        intros _. rewrite vec_change_neq. 2: intros ? % pos_right_inj; congruence.
+        rewrite vec_change_neq. 2: cbn; congruence.
+        rewrite vec_pos_set.
+        destruct cases as [ [ [| ] | ] | [q' Hq']]; rew vec.
+        exfalso. eapply pos_right_left. now rewrite Hq'. }
+      {  unfold vec_enc. rewrite !vec_pos_set.
+         destruct cases as [ [ [| ] | ] | [q Hq]]; rew vec.
+         { rewrite vec_pos_set. destruct cases as [ [ [| ] | ] | [q' Hq']]; rew vec.
+         exfalso. eapply pos_right_left. now rewrite Hq'. }
+         { rewrite vec_pos_set. destruct cases as [ [ [| ] | ] | [q' Hq']]; rew vec.
+         exfalso. eapply pos_right_left. now rewrite Hq'. }
+         { rewrite vec_change_neq. 2: intros ? % pos_right_inj % pos_nxt_inj; congruence.
+           rewrite vec_change_neq. 2: cbn; congruence.
+           rewrite vec_pos_set.
+           destruct cases as [ [ [| ] | ] | [q' Hq']]; rew vec.
+           exfalso. eapply pos_right_left. now rewrite Hq'. }
+      }
+      2:{  fold plus.
       mm sss stop. cbn. f_equal.
       rewrite cast_cast.
       reflexivity.
       }
-      cbn. autorewrite with list. setoid_rewrite PREP_length. lia.
+      {  unfold vec_enc. rewrite !vec_pos_set. destruct cases as [ [ [| ] | ] | [q' Hq']]; rew vec.
+         all: try now (cbn in e; congruence).
+         revert Hq'. eapply (Fin.caseS' q').
+         all: try now (cbn; congruence). }
+      Unshelve. lia.
+      }
+      cbn. autorewrite with list. cbn. setoid_rewrite PREPALL_length. right. lia.
+    + intros v H2.
+      eapply HP2. eapply HQ. eapply MM_cast_terminates with (E0 := E).
+      eapply subcode_sss_terminates.
+      2:{ eapply subcode_sss_terminates_inv. eapply mm_sss_fun.
+          eapply H2. 
+          2:{rewrite <- Eq1. rewrite <- MM_cast_spec.
+             rewrite PREPALL_length. cbn [plus].
+             match goal with [ |- sss_output _ _ _ (_, ?st) ] => evar (t : Vector.t nat (1 + k + i + 3)); enough (Eq : st = t) end; subst t.
+             rewrite Eq. eapply PREPALL_spec. 
+
+             clear.
+          eapply vec_pos_ext. intros p.
+          unfold vec_enc. rewrite vec_pos_set. destruct (cases p) as [ [[-> | ->] | ->] | [q ->]].
+          - cbn. rewrite <- !vec_app_spec. now rewrite vec_pos_app_right.
+          - cbn. rewrite <- !vec_app_spec. now rewrite vec_pos_app_right.
+          - cbn. rewrite <- !vec_app_spec. now rewrite vec_pos_app_right.
+          - rewrite <- !vec_app_spec. rewrite vec_pos_app_left.
+            revert q. eapply pos_left_right_rect.
+            + intros p. repeat setoid_rewrite vec_pos_app_left.
+              repeat setoid_rewrite <- vec_map_spec. eapply (Fin.caseS' p).
+              * cbn. reflexivity.
+              * intros. repeat setoid_rewrite vec_pos_map.
+                f_equal. rewrite (@vec_pos_app_left (list bool) (1 + k) i).
+                cbn. rewrite vec_pos_map. reflexivity.
+            + intros p. rewrite !vec_pos_app_right.
+              rewrite (@vec_pos_app_right (list bool) (S k) i).
+              now rewrite !vec_pos_const.
+          }
+ 
+      clear. subst q'. generalize (PREPALL k i 1).
+      intros l.
+      generalize (mm_transfert pos0 (pos_right (1 + k + i) pos2) (pos_right (1 + k + i) pos0) (1 + length l + length Q) ++ POSTP k i (4 + length l + length Q)).
+      fold plus. revert l. destruct E. cbn. intros. exists nil. cbn. eauto.
+      }
+
+      clear. subst q'.
+      generalize (PREPALL k i 1).
+      intros l.
+      generalize (mm_transfert pos0 (pos_right (1 + k + i) pos2) (pos_right (1 + k + i) pos0) (1 + length l + length Q) ++ POSTP k i (4 + length l + length Q)).
+      fold plus. revert l. destruct E. cbn. intros. exists l. cbn. eauto.
 Qed.
