theories/StackMachines/Util/BSM_computable.v
@@ -1,4 +1,4 @@
-Require Import Undecidability.StackMachines.BSM.
+From Undecidability Require Import BSM BSM_sss.
 
 From Coq Require Import List Vector.
 Import ListNotations Vector.VectorNotations.
@@ -9,3 +9,20 @@ Definition BSM_computable {k} (R : Vector.t nat k -> nat -> Prop) :=
       (forall m, R v m <->
          exists c v', BSM.eval (1 + k + n) (i, P) (i, (@List.nil bool :: Vector.map (fun n => List.repeat true n) v) ++ Vector.const (@List.nil bool) n) (c, List.repeat true m :: v'))
     /\ (forall c v', BSM.eval (1 + k + n) (i, P) (i, (@List.nil bool :: Vector.map (fun n => List.repeat true n) v) ++ Vector.const (@List.nil bool) n) (c, v') -> exists m v'', v' = List.repeat true m :: v'').    
+
+Lemma BSM_computable_iff {k} (R : Vector.t nat k -> nat -> Prop) :
+  BSM_computable R ->
+  exists n : nat, exists i : nat, exists P : list (bsm_instr (1 + k + n)),
+    (forall v : Vector.t nat k,forall m, R v m -> exists c v', BSM.eval (1 + k + n) (i, P) (i, (@List.nil bool :: Vector.map (fun n => List.repeat true n) v) ++ Vector.const (@List.nil bool) n) (c, List.repeat true m :: v'))
+    /\ (forall v, sss.sss_terminates (@bsm_sss _) (i, P) (i, (@List.nil bool :: Vector.map (fun n => List.repeat true n) v) ++ Vector.const (@List.nil bool) n) -> exists m, R v m).
+Proof.
+  intros (n & i & P & H). exists n, i, P. split.
+  - intros v m ? % H; eauto.
+  - intros v [(c, v') H1].
+    pose proof (H2 := H1). eapply eval_iff in H2 as (m & v'' & H2) % H.
+    subst. eapply eval_iff in H1. eexists. eapply H. eexists. eexists. eapply H1.
+Qed.
+
+    
+    
+    
